examples/tutorial/4-bir-to-arm/tutorial_bir_to_armScript.sml
@@ -47,7 +47,7 @@ val bir_add_reg_pre_def = Define `bir_add_reg_pre =
 `;
 
 val bir_add_reg_post_def = Define `bir_add_reg_post =
-(\(l:bir_label_t). (^(beq (bplus(get_y, get_x), get_ly))))`;
+ ^(beq (bplus(get_y, get_x), get_ly))`;
 
 
 val original_add_reg_loop_condition =  (bnot (bsle(get_lx, bconst64 0)));
@@ -79,7 +79,7 @@ val bir_add_reg_contract_1_pre_def = Define `bir_add_reg_contract_1_pre =
  (bir_add_reg_pre)
 `;
 val bir_add_reg_contract_1_post_def = Define `bir_add_reg_contract_1_post =
- (\(l:bir_label_t). (bir_add_reg_I))
+  bir_add_reg_I
 `;
 
 
@@ -89,7 +89,7 @@ val bir_add_reg_contract_2_pre_def = Define `bir_add_reg_contract_2_pre =
 ^(band(``bir_add_reg_I``, bir_add_reg_loop_condition))
 `;
 val bir_add_reg_contract_2_post_def = Define `bir_add_reg_contract_2_post =
- (\(l:bir_label_t). bir_add_reg_I)
+  bir_add_reg_I
 `;
 
 (* contract three: loop continue *)
@@ -98,7 +98,7 @@ val bir_add_reg_contract_3_pre_def = Define `bir_add_reg_contract_3_pre =
 ^(band(``bir_add_reg_I``, bir_add_reg_loop_condition))
 `;
 val bir_add_reg_contract_3_post_def = Define `bir_add_reg_contract_3_post =
- (\(l:bir_label_t). ^(band(``bir_add_reg_I``, bir_add_reg_loop_condition)))
+  ^(band(``bir_add_reg_I``, bir_add_reg_loop_condition))
 `;
 
 (* contract four: loop exit *)
@@ -123,10 +123,10 @@ val bir_add_reg_contract_2_pre_variant_def = Define `bir_add_reg_contract_2_pre_
 ])
 `;
 val bir_add_reg_contract_2_post_variant_def = Define `bir_add_reg_contract_2_post_variant v  =
- (\(l:bir_label_t). ^(bandl[``bir_add_reg_I``,
+ ^(bandl[``bir_add_reg_I``,
   bslt(get_lx, get_v),
   (bsle(bconst64 0, get_lx))
-]))
+])
 `;
 
 (* contract three: loop continue *)
@@ -135,7 +135,7 @@ val bir_add_reg_contract_3_pre_variant_def = Define `bir_add_reg_contract_3_pre_
 ^(bandl[``bir_add_reg_I``, bir_add_reg_loop_condition, beq(get_lx, get_v)])
 `;
 val bir_add_reg_contract_3_post_variant_def = Define `bir_add_reg_contract_3_post_variant v =
- (\(l:bir_label_t). ^(bandl[``bir_add_reg_I``, bir_add_reg_loop_condition, beq(get_lx, get_v)]))
+ ^(bandl[``bir_add_reg_I``, bir_add_reg_loop_condition, beq(get_lx, get_v)])
 `;
 
 
@@ -152,7 +152,7 @@ val bir_add_reg_contract_0_pre_def = Define `bir_add_reg_contract_0_pre =
 `;
 
 val bir_add_reg_contract_0_post_def = Define `bir_add_reg_contract_0_post =
-(\(l:bir_label_t). bir_add_reg_pre)
+bir_add_reg_pre
 `;
 
 
@@ -202,11 +202,11 @@ Cases_on `a < 0w` >> (
 
 val arm8_post_imp_bir_post_thm = store_thm("arm8_post_imp_bir_post_thm", 
   ``!(ls:bir_label_t -> bool).
-    bir_post_bir_to_arm8 arm8_add_reg_post bir_add_reg_post ls``,
+    bir_post_bir_to_arm8 arm8_add_reg_post (\(l:bir_label_t). bir_add_reg_post) ls``,
 
 FULL_SIMP_TAC std_ss [bir_post_bir_to_arm8_def] >>
 REPEAT STRIP_TAC >>
-UNDISCH_TAC ``bir_eval_exp (bir_add_reg_post l) bs.bst_environ = SOME bir_val_true`` >>
+UNDISCH_TAC ``bir_eval_exp bir_add_reg_post bs.bst_environ = SOME bir_val_true`` >>
 SIMP_TAC std_ss [bir_add_reg_post_def] >>
 SIMP_TAC std_ss arm_to_bir_exp_thms >>
 EVAL_TAC >>
