examples/tutorial/5-wp/tutorial_wpScript.sml
@@ -43,6 +43,17 @@ val _ = new_theory "tutorial_wp";
  * HT = Hoare triple
 *)
 
+val ending_lam_disj_to_sml_list = get_labels_from_lam_disj
+
+fun postcond_exp_from_label postcond label =
+  (snd o dest_eq o concl)
+    (SIMP_CONV
+      (bool_ss++HolBACoreSimps.holBACore_ss++wordsLib.WORD_ss) []
+      (mk_comb (postcond, label)
+    )
+  )
+;
+
 (******************************************************************)
                          (* New stuff *)
 (* Attempt at generating loop continuation contract with new
@@ -74,14 +85,7 @@ val test2 = EVAL test;
 val test3 = ((term_eq T) o snd o dest_eq o concl) test2
 
 *)
-fun postcond_exp_from_label postcond label =
-  (snd o dest_eq o concl)
-    (SIMP_CONV
-      (bool_ss++HolBACoreSimps.holBACore_ss++wordsLib.WORD_ss) []
-      (mk_comb (postcond, label)
-    )
-  )
-val ending_lam_disj_to_sml_list = get_labels_from_lam_disj
+
 
 (*
 val last_block_label_tm =  ``BL_Address (Imm64 0x20w)``; (* 32 *)
@@ -109,9 +113,9 @@ val bir_add_reg_contract_3_post_variant_def = Define `
 			  (BExp_Den (BVar "R2" (BType_Imm Bit64)))
 			  (BExp_Const (Imm64 v))))
 `;
-val postcond_tm = ``(\l. if (l = BL_Address (Imm64 0x20w))
+val postcond_tm = ``\l. if (l = BL_Address (Imm64 0x20w))
                          then bir_add_reg_contract_3_post_variant v
-                         else bir_exp_false)``;
+                         else bir_exp_false``;
 (* Postcondition for label? thm *)
 val test = SIMP_CONV bool_ss [] ``(^postcond_tm) (BL_Address (Imm64 0x20w))``
 (* defs is a list of theorems - typically definitions - which is
@@ -124,8 +128,8 @@ val defs = [bir_add_reg_prog_def, bir_add_reg_contract_3_post_variant_def,
             bir_add_reg_I_def, bir_exp_false_def, BType_Bool_def];
 val (bir_add_reg_new_loop_continue_variant_ht, bir_add_reg_new_loop_continue_variant_wp_tm) =
   bir_obtain_ht prog_tm first_block_label_tm ending_lam_disj
-    (ending_lam_disj_to_sml_list)
-                postcond_tm (postcond_exp_from_label) prefix defs;
+    ending_lam_disj_to_sml_list
+                postcond_tm postcond_exp_from_label prefix defs;
 (* By creating a definition and saving the HT as a theorem, we 
  * allow them to be exported to later theories. *)
 val bir_add_reg_new_loop_continue_variant_wp_def =
@@ -151,44 +155,18 @@ val prefix = "add_reg_entry_";
 (* This is the label of the "first block" in HT execution,
  * meaning the block at the beginning of which execution starts.  *)
 val first_block_label_tm = ``BL_Address (Imm64 0x1cw)``; (* 28 *)
-(* This is the last block of HT execution: the HT postcondition
- * (on the final state) is predicated on the state when this block
- * is reached.
- *
- * Note that in general, the HT execution could end when any label
- * out of a set of labels is reached. This would be the case for 
- * code which branches out to multiple exit points. Sets of ending
- * labels are supported by the current WP generation and proving
- * procedure, however different postconditions for different end
- * labels are not.
- *
- * For this exercise we will only treat single last block labels. *)
-val last_block_label_tm =  ``BL_Address (Imm64 0x40w)``; (* 64 *)
-(* TODO: Update this description to be in line with everything post-
- * new compositional HTs *)
-(* blacklist is a list of block labels, for which we assign
- * dummy HTs with False as pre- and postcondition.
- *
- * This can be hard to understand intuitively. First, consider a HT
- * with False as precondition. Since the first antecedent of the HT
- * would be that False holds, the conclusion always holds. This is
- * stated by the theorem bir_exec_to_labels_pre_F.
- *
- * Since HTs are generated incrementally from the end of execution
- * to the start, when a block which could jump to a block with dummy
- * HT is processed, the resulting HT would in effect be stating
- * the effect of execution assuming we do not jump to the block
- * with a dummy HT.
- *
- * Concretely, this is used in cases with conditional jumps, where
- * one of the jump targets signifies loop continuation. This allows
- * us to separately generate HTs for loop continuation and loop
- * exit, which we then can compose.  *)
-val blacklist = [];
+(* This is the Ending blocks of HT execution: the HT postcondition
+ * (on the final state) is predicated on the state when these blocks
+ * are reached. *)
+val ending_lam_disj =  ``\l.
+                         (l = BL_Address (Imm64 0x40w)) \/ (* 64 *)
+                         (l = BL_Address (Imm64 0x48w))``; (* 72 *)
 (* postcond_tm is the postcondition of the HT to be generated and
  * proved, which is obtained from the contract definitions in
  * tutorial_bir_to_armTheory. *)
-val postcond_tm = ``bir_add_reg_contract_1_post``;
+val postcond_tm = ``\l. if (l = BL_Address (Imm64 0x40w))
+                         then bir_add_reg_contract_1_post
+                         else bir_exp_false``;
 (* defs is a list of theorems - typically definitions - which is
  * used internally in bir_obtain_ht. This always contains the
  * program definition, the postcondition definition, and all other
@@ -196,7 +174,7 @@ val postcond_tm = ``bir_add_reg_contract_1_post``;
  * terms using only the syntax in the theory/bir directory of
  * HolBA. *)
 val defs = [bir_add_reg_prog_def, bir_add_reg_contract_1_post_def,
-            bir_add_reg_I_def, BType_Bool_def];
+            bir_add_reg_I_def, bir_exp_false_def, BType_Bool_def];
 
 (* Here, bir_obtain_ht is called with the above arguments.
  * bir_obtain_ht is a convenient wrapper function created for this
@@ -212,88 +190,16 @@ val defs = [bir_add_reg_prog_def, bir_add_reg_contract_1_post_def,
  * a list of theorems with definitions occuring inside the HT.
  * *)
 val (bir_add_reg_entry_ht, bir_add_reg_entry_wp_tm) =
-  bir_obtain_ht prog_tm first_block_label_tm last_block_label_tm
-                postcond_tm prefix blacklist defs;
+  bir_obtain_ht prog_tm first_block_label_tm
+                ending_lam_disj ending_lam_disj_to_sml_list
+                postcond_tm postcond_exp_from_label
+                prefix defs;
 (* By creating a definition and saving the HT as a theorem, we 
  * allow them to be exported to later theories. *)
 val bir_add_reg_entry_wp_def =
   Define `bir_add_reg_entry_wp = ^(bir_add_reg_entry_wp_tm)`;
 val _ = save_thm ("bir_add_reg_entry_ht", bir_add_reg_entry_ht);
 
-
-(****************    (2)  bir_add_reg_loop     ********************)
-(* The HT with the WP for the loop content of the add_reg program is
- * generated and proved here. *)
-(* 20 -> 24 -> 28 -> 2c -> 30 -> 34 -> 38 -> 3c -> 40 *)
-(* All of these arguments are analoguous to the ones in (1). *)
-val prefix = "add_reg_loop_";
-val first_block_label_tm = ``BL_Address (Imm64 0x20w)``;
-val last_block_label_tm =  ``BL_Address (Imm64 0x40w)``;
-val blacklist = [];
-val postcond_tm = ``bir_add_reg_contract_2_post``;
-val defs = [bir_add_reg_prog_def, bir_add_reg_contract_2_post_def,
-            bir_add_reg_I_def, BType_Bool_def];
-
-val (bir_add_reg_loop_ht, bir_add_reg_loop_wp_tm) =
-  bir_obtain_ht prog_tm first_block_label_tm last_block_label_tm
-                postcond_tm prefix blacklist defs;
-
-val bir_add_reg_loop_wp_def =
-  Define `bir_add_reg_loop_wp = ^(bir_add_reg_loop_wp_tm)`;
-val _ = save_thm ("bir_add_reg_loop_ht", bir_add_reg_loop_ht);
-
-(*************   (3)  bir_add_reg_loop_continue     ***************)
-(* This WP is for execution which starts at the loop condition and
- * then continues looping. *)
-(* 40 -> 20 *)
-val prefix = "add_reg_loop_continue_";
-val first_block_label_tm = ``BL_Address (Imm64 0x40w)``;
-val last_block_label_tm =  ``BL_Address (Imm64 0x20w)``;
-(* Here, we use the block label for 0x44 in blacklist. This
- * means that we are interested in the WP which describes execution
- * which does not proceed from 0x40 to 0x44, that is, exit the
- * loop. *)
-val blacklist = [``BL_Address (Imm64 0x44w)``];
-val postcond_tm = ``bir_add_reg_contract_3_post``;
-val defs = [bir_add_reg_prog_def, bir_add_reg_contract_3_post_def,
-            bir_add_reg_I_def, BType_Bool_def];
-
-val (bir_add_reg_loop_continue_ht,
-     bir_add_reg_loop_continue_wp_tm) =
-  bir_obtain_ht prog_tm first_block_label_tm last_block_label_tm
-                postcond_tm prefix blacklist defs;
-
-val bir_add_reg_loop_continue_wp_def = Define `
-  bir_add_reg_loop_continue_wp = ^(bir_add_reg_loop_continue_wp_tm)`
-;
-val _ =
-  save_thm ("bir_add_reg_loop_continue_ht",
-            bir_add_reg_loop_continue_ht);
-
-
-(**************    (4)   bir_add_reg_loop_exit      ***************)
-(* This WP is for execution which starts at the loop condition and
- * then exits the loop. Note that the blocks following 44 are
- * just SP manipulation and return. *)
-(* 40 -> 48 *)
-val prefix = "add_reg_loop_exit_";
-val first_block_label_tm = ``BL_Address (Imm64 0x40w)``;
-val last_block_label_tm =  ``BL_Address (Imm64 0x48w)``;
-(* In similar fashion as in (3), here we instead rule out loop
- * continuation. *)
-val blacklist = [``BL_Address (Imm64 0x20w)``];
-val postcond_tm = ``bir_add_reg_contract_4_post``;
-val defs = [bir_add_reg_prog_def, bir_add_reg_contract_4_post_def,
-            bir_add_reg_post_def];
-
-val (bir_add_reg_loop_exit_ht, bir_add_reg_loop_exit_wp_tm) =
-  bir_obtain_ht prog_tm first_block_label_tm last_block_label_tm
-                postcond_tm prefix blacklist defs;
-
-val bir_add_reg_loop_exit_wp_def = Define
-  `bir_add_reg_loop_exit_wp = ^(bir_add_reg_loop_exit_wp_tm)`;
-val _ =
-  save_thm ("bir_add_reg_loop_exit_ht", bir_add_reg_loop_exit_ht);
 
 (******************************************************************)
 (*                        LOOP VARIANT                            *)
@@ -319,23 +225,27 @@ val _ =
  * also require that the starting value is inside some valid range.
  * *)
 
-(**************    (2v)  bir_add_reg_loop_variant     *************)
+(**************    (2)  bir_add_reg_loop_variant     *************)
 (* The WP for the loop content is generated and proved here. This
  * is similar to (2) above. *)
 (* 20 -> 24 -> 28 -> 2c -> 30 -> 34 -> 38 -> 3c -> 40 *)
 val prefix = "add_reg_loop_variant_";
 val first_block_label_tm = ``BL_Address (Imm64 0x20w)``;
-val last_block_label_tm =  ``BL_Address (Imm64 0x40w)``;
-val blacklist = [];
-val postcond_tm =
-  ``bir_add_reg_contract_2_post_variant v``;
+val ending_lam_disj =  ``\l.
+                         (l = BL_Address (Imm64 0x40w)) \/ (* 64 *)
+                         (l = BL_Address (Imm64 0x48w))``; (* 72 *)
+val postcond_tm = ``\l. if (l = BL_Address (Imm64 0x20w))
+                         then bir_add_reg_contract_2_post_variant v
+                         else bir_exp_false``;
 val defs = [bir_add_reg_prog_def,
             bir_add_reg_contract_2_post_variant_def,
-            bir_add_reg_I_def, BType_Bool_def];
+            bir_add_reg_I_def, bir_exp_false_def, BType_Bool_def];
 
 val (bir_add_reg_loop_variant_ht, bir_add_reg_loop_variant_wp_tm) =
-  bir_obtain_ht prog_tm first_block_label_tm last_block_label_tm
-                postcond_tm prefix blacklist defs;
+  bir_obtain_ht prog_tm first_block_label_tm
+                ending_lam_disj ending_lam_disj_to_sml_list
+                postcond_tm postcond_exp_from_label
+                prefix defs;
 
 val bir_add_reg_loop_variant_wp_def = Define `
   bir_add_reg_loop_variant_wp v =
@@ -345,23 +255,29 @@ val _ = save_thm ("bir_add_reg_loop_variant_ht",
                   bir_add_reg_loop_variant_ht);
 
 
-(*********   (3v)  bir_add_reg_loop_continue_variant     **********)
+(*********   (3)  bir_add_reg_loop_continue_variant     **********)
 (* This WP is for execution which starts at the loop condition and
  * then continues looping. *)
 (* 40 -> 20 *)
 val prefix = "add_reg_loop_continue_variant_";
 val first_block_label_tm = ``BL_Address (Imm64 0x40w)``;
-val last_block_label_tm =  ``BL_Address (Imm64 0x20w)``;
-val blacklist = [``BL_Address (Imm64 0x44w)``];
-val postcond_tm = ``bir_add_reg_contract_3_post_variant v``;
+val ending_lam_disj = ``\l.
+                        (l = BL_Address (Imm64 0x20w)) \/
+                        (l = BL_Address (Imm64 0x40w)) \/
+                        (l = BL_Address (Imm64 0x48w))``;
+val postcond_tm = ``\l. if (l = BL_Address (Imm64 0x20w))
+                         then bir_add_reg_contract_3_post_variant v
+                         else bir_exp_false``;
 val defs = [bir_add_reg_prog_def,
             bir_add_reg_contract_3_post_variant_def,
-            bir_add_reg_I_def, BType_Bool_def];
+            bir_add_reg_I_def, bir_exp_false_def, BType_Bool_def];
 
 val (bir_add_reg_loop_continue_variant_ht,
      bir_add_reg_loop_continue_variant_wp_tm) =
-  bir_obtain_ht prog_tm first_block_label_tm last_block_label_tm
-                postcond_tm prefix blacklist defs;
+  bir_obtain_ht prog_tm first_block_label_tm
+                ending_lam_disj ending_lam_disj_to_sml_list
+                postcond_tm postcond_exp_from_label
+                prefix defs;
 
 val bir_add_reg_loop_continue_variant_wp_def = Define `
   bir_add_reg_loop_continue_variant_wp v =
@@ -369,6 +285,35 @@ val bir_add_reg_loop_continue_variant_wp_def = Define `
 `;
 val _ = save_thm ("bir_add_reg_loop_continue_variant_ht",
                   bir_add_reg_loop_continue_variant_ht);
+
+
+(**************    (4)   bir_add_reg_loop_exit      ***************)
+(* This WP is for execution which starts at the loop condition and
+ * then exits the loop. Note that the blocks following 44 are
+ * just SP manipulation and return. *)
+(* 40 -> 48 *)
+val prefix = "add_reg_loop_exit_";
+val first_block_label_tm = ``BL_Address (Imm64 0x40w)``;
+val ending_lam_disj = ``\l.
+                        (l = BL_Address (Imm64 0x20w)) \/
+                        (l = BL_Address (Imm64 0x48w))``;
+val postcond_tm = ``\l. if (l = BL_Address (Imm64 0x48w))
+                         then bir_add_reg_contract_4_post
+                         else bir_exp_false``;
+val defs = [bir_add_reg_prog_def, bir_add_reg_contract_4_post_def,
+            bir_add_reg_post_def, bir_exp_false_def];
+
+val (bir_add_reg_loop_exit_ht, bir_add_reg_loop_exit_wp_tm) =
+  bir_obtain_ht prog_tm first_block_label_tm
+                ending_lam_disj ending_lam_disj_to_sml_list
+                postcond_tm postcond_exp_from_label
+                prefix defs;
+
+val bir_add_reg_loop_exit_wp_def = Define
+  `bir_add_reg_loop_exit_wp = ^(bir_add_reg_loop_exit_wp_tm)`;
+val _ =
+  save_thm ("bir_add_reg_loop_exit_ht", bir_add_reg_loop_exit_ht);
+
 
 (************            SOME EXPERIMENTS            **************)
 (* What about the preamble of the function, where the arguments are
@@ -390,14 +335,14 @@ val _ = save_thm ("bir_add_reg_loop_continue_variant_ht",
 (*
 val prefix = "add_reg_mem_";
 val first_block_label_tm = ``BL_Address (Imm64 0x0w)``; (* 28 *)
-val last_block_label_tm =  ``BL_Address (Imm64 0x1cw)``; (* 64 *)
+val ending_lam_disj =  ``BL_Address (Imm64 0x1cw)``; (* 64 *)
 val blacklist = [];
 val postcond_tm = ``bir_add_reg_contract_0_post``;
 val defs = [bir_add_reg_prog_def, bir_add_reg_contract_0_post_def,
             bir_add_reg_contract_0_pre_def];
 
 val (bir_add_reg_mem_ht, bir_add_reg_mem_wp_tm) =
-  bir_obtain_ht prog_tm first_block_label_tm last_block_label_tm
+  bir_obtain_ht prog_tm first_block_label_tm ending_lam_disj
                 postcond_tm prefix blacklist defs;
 
 val bir_add_reg_mem_wp_def = Define `
